<?xml version="1.0"?>
<rdf:RDF xmlns="http://www.semanticweb.org/walte/ontologies/2024/5/Hedgehog_Dilemma/"
     xml:base="http://www.semanticweb.org/walte/ontologies/2024/5/Hedgehog_Dilemma/"
     xmlns:dc="http://purl.org/dc/elements/1.1/"
     xmlns:owl="http://www.w3.org/2002/07/owl#"
     xmlns:rdf="http://www.w3.org/1999/02/22-rdf-syntax-ns#"
     xmlns:xml="http://www.w3.org/XML/1998/namespace"
     xmlns:xsd="http://www.w3.org/2001/XMLSchema#"
     xmlns:rdfs="http://www.w3.org/2000/01/rdf-schema#"
     xmlns:sequence="http://www.ontologydesignpatterns.org/cp/owl/sequence.owl#"
     xmlns:taskrole="http://www.ontologydesignpatterns.org/cp/owl/taskrole.owl#"
     xmlns:coredilemma="http://www.ontologydesignpatterns.org/ont/dilemmas/coredilemma.owl#"
     xmlns:description="http://www.ontologydesignpatterns.org/cp/owl/description.owl#"
     xmlns:Hedgehog_Dilemma="http://www.semanticweb.org/walte/ontologies/2024/5/Hedgehog_Dilemma#"
     xmlns:Hedgehog_Dilemma9="http://www.semanticweb.org/walte/ontologies/2024/5/Hedgehog_Dilemma9#"
     xmlns:cpannotationschema="http://www.ontologydesignpatterns.org/schemas/cpannotationschema.owl#"
     xmlns:untitled-ontology-9="http://www.semanticweb.org/walte/ontologies/2024/5/untitled-ontology-9#"
     xmlns:descriptionandsituation="http://www.ontologydesignpatterns.org/cp/owl/descriptionandsituation.owl#">
    <owl:Ontology rdf:about="http://www.semanticweb.org/walte/ontologies/2024/5/Hedgehog_Dilemma">
        <owl:imports rdf:resource="http://www.ontologydesignpatterns.org/ont/dilemmas/coredilemma.owl"/>
        <rdfs:comment>This ontology represents the Hedgehog Dilemma, firstly formulated from Artur Schopenhauer in his &quot;Parerga and Paralipomena&quot;, when he points out a rapresentation of the human&apos;s interactions: &quot;One cold winter&apos;s day, a number of porcupines huddled together quite closely in order through their mutual warmth to prevent themselves from being frozen. But they soon felt the effect of their quills on one another, which made them again move apart. Now when the need for warmth once more brought them together, the drawback of the quills was repeated so that they were tossed between two evils, until they had discovered the proper distance from which they could best tolerate one another. Thus the need for society which springs from the emptiness and monotony of men&apos;s lives, drives them together; but their many unpleasant and repulsive qualities and insufferable drawbacks once more drive them apart. The mean distance which they finally discover, and which enables them to endure being together, is politeness and good manners. Whoever does not keep to this, is told in England to ‘keep his distance’. By virtue thereof, it is true that the need for mutual warmth will be only imperfectly satisfied, but on the other hand, the prick of the quills will not be felt. Yet whoever has a great deal of internal warmth of his own will prefer to keep away from society in order to avoid giving or receiving trouble or annoyance.&quot;.

When it comes to present a real situation, I used a study from Maner and colleagues where they analyze social exclusion from the example of the Hedgehog Dilemma, describeing how people respond to being excluded from society. What they do are some experiments inside groups of people, each with a different focus, showing, in the end, the complexity of the situation: result shows a common desire to renew affiliative bonds after being excluded, but carefoully, because rejected people want to protect themselves, pointing out some boundary condictions. 
Here&apos;s the paper&apos;s summary: &quot;Evidence from 6 experiments supports the social reconnection hypothesis, which posits that the experience of social exclusion increases the motivation to forge social bonds with new sources of potential affiliation. Threat of social exclusion led participants to express greater interest in making new friends, to increase their desire to work with others, to form more positive impressions of novel social targets, and to assign greater rewards to new interaction partners. Findings also suggest potential boundary conditions to the social reconnection hypothesis. Excluded individuals did not seem to seek reconnection with the specific perpetrators of exclusion or with novel partners with whom no face-to-face interaction was anticipated. Furthermore, fear of negative evaluation moderated responses to exclusion such that participants low in fear of negative evaluation responded to new interaction partners in an affiliative fashion, whereas participants high in fear of negative evaluation did not.&quot;. 

For this ontology, I apply the experiment number 4, where it&apos;s analyzed the relation between a rejecter person and their rejector.</rdfs:comment>
    </owl:Ontology>
    


    <!-- 
    ///////////////////////////////////////////////////////////////////////////////////////
    //
    // Object Properties
    //
    ///////////////////////////////////////////////////////////////////////////////////////
     -->

    


    <!-- http://www.semanticweb.org/walte/ontologies/2024/5/Hedgehog_Dilemma#hasOption -->

    <owl:ObjectProperty rdf:about="http://www.semanticweb.org/walte/ontologies/2024/5/Hedgehog_Dilemma#hasOption">
        <rdfs:subPropertyOf rdf:resource="http://www.w3.org/2002/07/owl#topObjectProperty"/>
        <rdfs:domain rdf:resource="http://www.ontologydesignpatterns.org/cp/owl/taskrole.owl#Task"/>
        <rdfs:range rdf:resource="http://www.ontologydesignpatterns.org/ont/dilemmas/coredilemma.owl#Criterion"/>
        <dc:creator>Walter Bertoli</dc:creator>
    </owl:ObjectProperty>
    


    <!-- http://www.semanticweb.org/walte/ontologies/2024/5/Hedgehog_Dilemma9#hasCriterion -->

    <owl:ObjectProperty rdf:about="http://www.semanticweb.org/walte/ontologies/2024/5/Hedgehog_Dilemma9#hasCriterion">
        <rdfs:domain rdf:resource="http://www.ontologydesignpatterns.org/cp/owl/description.owl#Description"/>
        <rdfs:domain rdf:resource="http://www.ontologydesignpatterns.org/ont/dilemmas/coredilemma.owl#Outcome"/>
        <rdfs:range rdf:resource="http://www.ontologydesignpatterns.org/ont/dilemmas/coredilemma.owl#Criterion"/>
        <dc:creator>Walter Bertoli</dc:creator>
    </owl:ObjectProperty>
    


    <!-- 
    ///////////////////////////////////////////////////////////////////////////////////////
    //
    // Data properties
    //
    ///////////////////////////////////////////////////////////////////////////////////////
     -->

    


    <!-- http://www.semanticweb.org/walte/ontologies/2024/5/Hedgehog_Dilemma#Temperature -->

    <owl:DatatypeProperty rdf:about="http://www.semanticweb.org/walte/ontologies/2024/5/Hedgehog_Dilemma#Temperature">
        <rdfs:subPropertyOf rdf:resource="http://www.w3.org/2002/07/owl#topDataProperty"/>
        <rdfs:domain rdf:resource="http://www.ontologydesignpatterns.org/cp/owl/controlflow.owl#DecisionActivity"/>
        <dc:creator>Walter Bertoli</dc:creator>
        <rdfs:comment>Each hedgehog has its own temperature. 
If it is &gt;20, the hedgehog will search contact with other animals to rise its temperature.</rdfs:comment>
    </owl:DatatypeProperty>
    


    <!-- 
    ///////////////////////////////////////////////////////////////////////////////////////
    //
    // Classes
    //
    ///////////////////////////////////////////////////////////////////////////////////////
     -->

    


    <!-- http://www.ontologydesignpatterns.org/ont/dilemmas/coredilemma.owl#Criterion -->

    <rdf:Description rdf:about="http://www.ontologydesignpatterns.org/ont/dilemmas/coredilemma.owl#Criterion">
        <rdfs:subClassOf>
            <owl:Restriction>
                <owl:onProperty rdf:resource="http://www.ontologydesignpatterns.org/ont/dilemmas/coredilemma.owl#hasOutcome"/>
                <owl:someValuesFrom rdf:resource="http://www.ontologydesignpatterns.org/ont/dilemmas/coredilemma.owl#Outcome"/>
            </owl:Restriction>
        </rdfs:subClassOf>
    </rdf:Description>
    


    <!-- http://www.ontologydesignpatterns.org/ont/dilemmas/coredilemma.owl#Outcome -->

    <rdf:Description rdf:about="http://www.ontologydesignpatterns.org/ont/dilemmas/coredilemma.owl#Outcome">
        <rdfs:subClassOf>
            <owl:Restriction>
                <owl:onProperty rdf:resource="http://www.semanticweb.org/walte/ontologies/2024/5/Hedgehog_Dilemma9#hasCriterion"/>
                <owl:someValuesFrom rdf:resource="http://www.ontologydesignpatterns.org/ont/dilemmas/coredilemma.owl#Criterion"/>
            </owl:Restriction>
        </rdfs:subClassOf>
    </rdf:Description>
    


    <!-- http://www.semanticweb.org/walte/ontologies/2024/5/Hedgehog_Dilemma9#GetCloser -->

    <owl:Class rdf:about="http://www.semanticweb.org/walte/ontologies/2024/5/Hedgehog_Dilemma9#GetCloser">
        <rdfs:subClassOf rdf:resource="http://www.ontologydesignpatterns.org/ont/dilemmas/coredilemma.owl#Outcome"/>
        <owl:disjointWith rdf:resource="http://www.semanticweb.org/walte/ontologies/2024/5/Hedgehog_Dilemma9#MoveAway"/>
        <owl:disjointWith rdf:resource="http://www.semanticweb.org/walte/ontologies/2024/5/Hedgehog_Dilemma9#ProperDistance"/>
    </owl:Class>
    


    <!-- http://www.semanticweb.org/walte/ontologies/2024/5/Hedgehog_Dilemma9#HedgehogSituation -->

    <owl:Class rdf:about="http://www.semanticweb.org/walte/ontologies/2024/5/Hedgehog_Dilemma9#HedgehogSituation">
        <rdfs:subClassOf rdf:resource="http://www.ontologydesignpatterns.org/ont/dilemmas/coredilemma.owl#DilemmaticSituation"/>
        <dc:creator>Walter Bertoli</dc:creator>
    </owl:Class>
    


    <!-- http://www.semanticweb.org/walte/ontologies/2024/5/Hedgehog_Dilemma9#HedgehogTask -->

    <owl:Class rdf:about="http://www.semanticweb.org/walte/ontologies/2024/5/Hedgehog_Dilemma9#HedgehogTask">
        <rdfs:subClassOf rdf:resource="http://www.ontologydesignpatterns.org/cp/owl/taskrole.owl#Task"/>
        <dc:creator>Walter Bertoli</dc:creator>
    </owl:Class>
    


    <!-- http://www.semanticweb.org/walte/ontologies/2024/5/Hedgehog_Dilemma9#Hedgehogs -->

    <owl:Class rdf:about="http://www.semanticweb.org/walte/ontologies/2024/5/Hedgehog_Dilemma9#Hedgehogs">
        <owl:equivalentClass rdf:resource="http://www.semanticweb.org/walte/ontologies/2024/5/Hedgehog_Dilemma9#Humans"/>
        <rdfs:subClassOf rdf:resource="http://www.ontologydesignpatterns.org/cp/owl/agentrole.owl#Agent"/>
        <dc:creator>Walter Bertoli</dc:creator>
    </owl:Class>
    


    <!-- http://www.semanticweb.org/walte/ontologies/2024/5/Hedgehog_Dilemma9#Humans -->

    <owl:Class rdf:about="http://www.semanticweb.org/walte/ontologies/2024/5/Hedgehog_Dilemma9#Humans">
        <rdfs:subClassOf rdf:resource="http://www.ontologydesignpatterns.org/cp/owl/classification.owl#Concept"/>
        <dc:creator>Walter Bertoli</dc:creator>
        <rdfs:comment>The Hedgehog Dilemma is a metaphora for the human&apos;s social relations</rdfs:comment>
    </owl:Class>
    


    <!-- http://www.semanticweb.org/walte/ontologies/2024/5/Hedgehog_Dilemma9#Individualism -->

    <owl:Class rdf:about="http://www.semanticweb.org/walte/ontologies/2024/5/Hedgehog_Dilemma9#Individualism">
        <rdfs:subClassOf rdf:resource="http://www.ontologydesignpatterns.org/ont/dilemmas/coredilemma.owl#Criterion"/>
        <owl:disjointWith rdf:resource="http://www.semanticweb.org/walte/ontologies/2024/5/Hedgehog_Dilemma9#Interdependence"/>
        <owl:disjointWith rdf:resource="http://www.semanticweb.org/walte/ontologies/2024/5/Hedgehog_Dilemma9#Kindness"/>
    </owl:Class>
    


    <!-- http://www.semanticweb.org/walte/ontologies/2024/5/Hedgehog_Dilemma9#Interdependence -->

    <owl:Class rdf:about="http://www.semanticweb.org/walte/ontologies/2024/5/Hedgehog_Dilemma9#Interdependence">
        <rdfs:subClassOf rdf:resource="http://www.ontologydesignpatterns.org/ont/dilemmas/coredilemma.owl#Criterion"/>
        <owl:disjointWith rdf:resource="http://www.semanticweb.org/walte/ontologies/2024/5/Hedgehog_Dilemma9#Kindness"/>
    </owl:Class>
    


    <!-- http://www.semanticweb.org/walte/ontologies/2024/5/Hedgehog_Dilemma9#Kindness -->

    <owl:Class rdf:about="http://www.semanticweb.org/walte/ontologies/2024/5/Hedgehog_Dilemma9#Kindness">
        <rdfs:subClassOf rdf:resource="http://www.ontologydesignpatterns.org/ont/dilemmas/coredilemma.owl#Criterion"/>
    </owl:Class>
    


    <!-- http://www.semanticweb.org/walte/ontologies/2024/5/Hedgehog_Dilemma9#MoveAway -->

    <owl:Class rdf:about="http://www.semanticweb.org/walte/ontologies/2024/5/Hedgehog_Dilemma9#MoveAway">
        <rdfs:subClassOf rdf:resource="http://www.ontologydesignpatterns.org/ont/dilemmas/coredilemma.owl#Outcome"/>
        <owl:disjointWith rdf:resource="http://www.semanticweb.org/walte/ontologies/2024/5/Hedgehog_Dilemma9#ProperDistance"/>
    </owl:Class>
    


    <!-- http://www.semanticweb.org/walte/ontologies/2024/5/Hedgehog_Dilemma9#ProperDistance -->

    <owl:Class rdf:about="http://www.semanticweb.org/walte/ontologies/2024/5/Hedgehog_Dilemma9#ProperDistance">
        <rdfs:subClassOf rdf:resource="http://www.ontologydesignpatterns.org/ont/dilemmas/coredilemma.owl#Outcome"/>
    </owl:Class>
    


    <!-- 
    ///////////////////////////////////////////////////////////////////////////////////////
    //
    // Individuals
    //
    ///////////////////////////////////////////////////////////////////////////////////////
     -->

    


    <!-- http://www.semanticweb.org/walte/ontologies/2024/5/Hedgehog_Dilemma#ChooseMoralValue -->

    <owl:NamedIndividual rdf:about="http://www.semanticweb.org/walte/ontologies/2024/5/Hedgehog_Dilemma#ChooseMoralValue">
        <rdf:type rdf:resource="http://www.ontologydesignpatterns.org/cp/owl/controlflow.owl#CaseTask"/>
        <sequence:follows rdf:resource="http://www.semanticweb.org/walte/ontologies/2024/5/Hedgehog_Dilemma#Evaluate_Conditions"/>
        <sequence:precedes rdf:resource="http://www.semanticweb.org/walte/ontologies/2024/5/Hedgehog_Dilemma#EvaluateOptions"/>
        <Hedgehog_Dilemma:hasOption rdf:resource="http://www.semanticweb.org/walte/ontologies/2024/5/Hedgehog_Dilemma9#Individualism"/>
        <Hedgehog_Dilemma:hasOption rdf:resource="http://www.semanticweb.org/walte/ontologies/2024/5/Hedgehog_Dilemma9#Interdependence"/>
        <Hedgehog_Dilemma:hasOption rdf:resource="http://www.semanticweb.org/walte/ontologies/2024/5/Hedgehog_Dilemma9#Kindness"/>
        <rdfs:comment>The Hedgehog decide which criterion will drive its decisions.</rdfs:comment>
    </owl:NamedIndividual>
    


    <!-- http://www.semanticweb.org/walte/ontologies/2024/5/Hedgehog_Dilemma#EvaluateOptions -->

    <owl:NamedIndividual rdf:about="http://www.semanticweb.org/walte/ontologies/2024/5/Hedgehog_Dilemma#EvaluateOptions">
        <rdf:type rdf:resource="http://www.ontologydesignpatterns.org/cp/owl/controlflow.owl#DeliberationTask"/>
        <owl:differentFrom rdf:resource="http://www.semanticweb.org/walte/ontologies/2024/5/Hedgehog_Dilemma#Evaluate_Conditions"/>
        <owl:differentFrom rdf:resource="http://www.semanticweb.org/walte/ontologies/2024/5/Hedgehog_Dilemma#ExploreOptions"/>
        <sequence:follows rdf:resource="http://www.semanticweb.org/walte/ontologies/2024/5/Hedgehog_Dilemma#ChooseMoralValue"/>
        <sequence:precedes rdf:resource="http://www.semanticweb.org/walte/ontologies/2024/5/Hedgehog_Dilemma#ExploreOptions"/>
        <rdfs:comment>Once the moral values have been chosen, the Hedgehog analyzes and plans the situation, evaluateing the distance it wants to take.</rdfs:comment>
    </owl:NamedIndividual>
    


    <!-- http://www.semanticweb.org/walte/ontologies/2024/5/Hedgehog_Dilemma#Evaluate_Conditions -->

    <owl:NamedIndividual rdf:about="http://www.semanticweb.org/walte/ontologies/2024/5/Hedgehog_Dilemma#Evaluate_Conditions">
        <rdf:type rdf:resource="http://www.ontologydesignpatterns.org/cp/owl/controlflow.owl#ActivationTask"/>
        <owl:differentFrom rdf:resource="http://www.semanticweb.org/walte/ontologies/2024/5/Hedgehog_Dilemma#ExploreOptions"/>
        <sequence:follows rdf:resource="http://www.semanticweb.org/walte/ontologies/2024/5/Hedgehog_Dilemma9#BeingAlone_and_Pain"/>
        <sequence:precedes rdf:resource="http://www.semanticweb.org/walte/ontologies/2024/5/Hedgehog_Dilemma#ChooseMoralValue"/>
        <dc:creator>Walter Bertoli</dc:creator>
        <rdfs:comment>Being in a Pain and Cold state (the DecisionState), the Hedgehog begins to evaluate the phisical external conditions.</rdfs:comment>
    </owl:NamedIndividual>
    


    <!-- http://www.semanticweb.org/walte/ontologies/2024/5/Hedgehog_Dilemma#ExploreOptions -->

    <owl:NamedIndividual rdf:about="http://www.semanticweb.org/walte/ontologies/2024/5/Hedgehog_Dilemma#ExploreOptions">
        <rdf:type rdf:resource="http://www.ontologydesignpatterns.org/cp/owl/controlflow.owl#ConcurrencyTask"/>
        <sequence:follows rdf:resource="http://www.semanticweb.org/walte/ontologies/2024/5/Hedgehog_Dilemma#EvaluateOptions"/>
        <sequence:precedes rdf:resource="http://www.semanticweb.org/walte/ontologies/2024/5/Hedgehog_Dilemma#StabilizePosition"/>
        <dc:creator>Walter Bertoli</dc:creator>
        <rdfs:comment>The Hedgehog explores simultaneously all of the options, considering wich movement to take.</rdfs:comment>
    </owl:NamedIndividual>
    


    <!-- http://www.semanticweb.org/walte/ontologies/2024/5/Hedgehog_Dilemma#FeelGood -->

    <owl:NamedIndividual rdf:about="http://www.semanticweb.org/walte/ontologies/2024/5/Hedgehog_Dilemma#FeelGood">
        <rdf:type rdf:resource="http://www.ontologydesignpatterns.org/cp/owl/controlflow.owl#EndingTask"/>
        <sequence:follows rdf:resource="http://www.semanticweb.org/walte/ontologies/2024/5/Hedgehog_Dilemma#Movement"/>
        <rdfs:comment>To complete the dilemma, the Hedgehog has to feel good, applying his choices and values in order to find its place in the ralations with others</rdfs:comment>
    </owl:NamedIndividual>
    


    <!-- http://www.semanticweb.org/walte/ontologies/2024/5/Hedgehog_Dilemma#Hedgehog1 -->

    <owl:NamedIndividual rdf:about="http://www.semanticweb.org/walte/ontologies/2024/5/Hedgehog_Dilemma#Hedgehog1">
        <rdf:type rdf:resource="http://www.ontologydesignpatterns.org/cp/owl/objectrole.owl#Role"/>
        <rdf:type rdf:resource="http://www.ontologydesignpatterns.org/cp/owl/taskrole.owl#Role"/>
        <owl:differentFrom rdf:resource="http://www.semanticweb.org/walte/ontologies/2024/5/Hedgehog_Dilemma#Hedgehog2"/>
        <descriptionandsituation:isDescribedBy rdf:resource="http://www.semanticweb.org/walte/ontologies/2024/5/Hedgehog_Dilemma9#Individualism"/>
        <taskrole:hasTask rdf:resource="http://www.semanticweb.org/walte/ontologies/2024/5/Hedgehog_Dilemma#Movement"/>
    </owl:NamedIndividual>
    


    <!-- http://www.semanticweb.org/walte/ontologies/2024/5/Hedgehog_Dilemma#Hedgehog2 -->

    <owl:NamedIndividual rdf:about="http://www.semanticweb.org/walte/ontologies/2024/5/Hedgehog_Dilemma#Hedgehog2">
        <rdf:type rdf:resource="http://www.ontologydesignpatterns.org/cp/owl/objectrole.owl#Role"/>
        <rdf:type rdf:resource="http://www.ontologydesignpatterns.org/cp/owl/taskrole.owl#Role"/>
        <descriptionandsituation:isDescribedBy rdf:resource="http://www.semanticweb.org/walte/ontologies/2024/5/Hedgehog_Dilemma9#Interdependence"/>
        <taskrole:hasTask rdf:resource="http://www.semanticweb.org/walte/ontologies/2024/5/Hedgehog_Dilemma#Movement"/>
    </owl:NamedIndividual>
    


    <!-- http://www.semanticweb.org/walte/ontologies/2024/5/Hedgehog_Dilemma#Movement -->

    <owl:NamedIndividual rdf:about="http://www.semanticweb.org/walte/ontologies/2024/5/Hedgehog_Dilemma#Movement">
        <rdf:type rdf:resource="http://www.ontologydesignpatterns.org/cp/owl/controlflow.owl#ActionTask"/>
        <sequence:follows rdf:resource="http://www.semanticweb.org/walte/ontologies/2024/5/Hedgehog_Dilemma#StabilizePosition"/>
        <sequence:precedes rdf:resource="http://www.semanticweb.org/walte/ontologies/2024/5/Hedgehog_Dilemma#FeelGood"/>
        <taskrole:isTaskOf rdf:resource="http://www.semanticweb.org/walte/ontologies/2024/5/Hedgehog_Dilemma#Hedgehog1"/>
        <taskrole:isTaskOf rdf:resource="http://www.semanticweb.org/walte/ontologies/2024/5/Hedgehog_Dilemma#Hedgehog2"/>
        <coredilemma:causallyLinkedTo rdf:resource="http://www.semanticweb.org/walte/ontologies/2024/5/Hedgehog_Dilemma9#GetCloser"/>
        <coredilemma:causallyLinkedTo rdf:resource="http://www.semanticweb.org/walte/ontologies/2024/5/Hedgehog_Dilemma9#MoveAway"/>
        <coredilemma:causallyLinkedTo rdf:resource="http://www.semanticweb.org/walte/ontologies/2024/5/Hedgehog_Dilemma9#ProperDistance"/>
        <rdfs:comment>In order to realize its decision the Hedgehog has to implement movement. Here the animal sequences a non-planning activity, which is an automatic activity that doesn&apos;t involve a rational event.</rdfs:comment>
    </owl:NamedIndividual>
    


    <!-- http://www.semanticweb.org/walte/ontologies/2024/5/Hedgehog_Dilemma#StabilizePosition -->

    <owl:NamedIndividual rdf:about="http://www.semanticweb.org/walte/ontologies/2024/5/Hedgehog_Dilemma#StabilizePosition">
        <rdf:type rdf:resource="http://www.ontologydesignpatterns.org/cp/owl/controlflow.owl#SynchroTask"/>
        <sequence:follows rdf:resource="http://www.semanticweb.org/walte/ontologies/2024/5/Hedgehog_Dilemma#ExploreOptions"/>
        <sequence:precedes rdf:resource="http://www.semanticweb.org/walte/ontologies/2024/5/Hedgehog_Dilemma#Movement"/>
        <dc:creator>Walter Bertoli</dc:creator>
        <rdfs:comment>In the synchro task the Hedgehog gets imputs from the Concurrency task, coordinateing the various actions to get the right balance between pain and heat according to the decision made and the criterion used</rdfs:comment>
    </owl:NamedIndividual>
    


    <!-- http://www.semanticweb.org/walte/ontologies/2024/5/Hedgehog_Dilemma9#BeingAlone_and_Pain -->

    <owl:NamedIndividual rdf:about="http://www.semanticweb.org/walte/ontologies/2024/5/Hedgehog_Dilemma9#BeingAlone_and_Pain">
        <rdf:type rdf:resource="http://www.ontologydesignpatterns.org/cp/owl/controlflow.owl#DeliberationState"/>
        <owl:differentFrom rdf:resource="http://www.semanticweb.org/walte/ontologies/2024/5/Hedgehog_Dilemma9#Coldness"/>
        <owl:differentFrom rdf:resource="http://www.semanticweb.org/walte/ontologies/2024/5/Hedgehog_Dilemma9#GetHurt"/>
        <owl:differentFrom rdf:resource="http://www.semanticweb.org/walte/ontologies/2024/5/Hedgehog_Dilemma9#MoveCloser"/>
        <sequence:follows rdf:resource="http://www.semanticweb.org/walte/ontologies/2024/5/Hedgehog_Dilemma9#GetHurt"/>
        <sequence:precedes rdf:resource="http://www.semanticweb.org/walte/ontologies/2024/5/Hedgehog_Dilemma#Evaluate_Conditions"/>
        <dc:creator>Walter Bertoli</dc:creator>
        <rdfs:comment>The Hedgehog, after it has experienced coldness and pain, is in a state between being alone and mental pain. Now it is in the situation to choose what to do.</rdfs:comment>
    </owl:NamedIndividual>
    


    <!-- http://www.semanticweb.org/walte/ontologies/2024/5/Hedgehog_Dilemma9#Coldness -->

    <owl:NamedIndividual rdf:about="http://www.semanticweb.org/walte/ontologies/2024/5/Hedgehog_Dilemma9#Coldness">
        <rdf:type rdf:resource="http://www.ontologydesignpatterns.org/cp/owl/controlflow.owl#DecisionActivity"/>
        <owl:differentFrom rdf:resource="http://www.semanticweb.org/walte/ontologies/2024/5/Hedgehog_Dilemma9#GetHurt"/>
        <owl:differentFrom rdf:resource="http://www.semanticweb.org/walte/ontologies/2024/5/Hedgehog_Dilemma9#MoveCloser"/>
        <sequence:precedes rdf:resource="http://www.semanticweb.org/walte/ontologies/2024/5/Hedgehog_Dilemma9#MoveCloser"/>
        <Hedgehog_Dilemma:Temperature rdf:datatype="http://www.w3.org/2001/XMLSchema#decimal">15</Hedgehog_Dilemma:Temperature>
        <dc:creator>Walter Bertoli</dc:creator>
        <rdfs:comment>The Hedgehod fells coldness: it is alone and without heat sources.</rdfs:comment>
    </owl:NamedIndividual>
    


    <!-- http://www.semanticweb.org/walte/ontologies/2024/5/Hedgehog_Dilemma9#GetCloser -->

    <owl:NamedIndividual rdf:about="http://www.semanticweb.org/walte/ontologies/2024/5/Hedgehog_Dilemma9#GetCloser">
        <rdf:type rdf:resource="http://www.semanticweb.org/walte/ontologies/2024/5/Hedgehog_Dilemma9#GetCloser"/>
        <owl:differentFrom rdf:resource="http://www.semanticweb.org/walte/ontologies/2024/5/Hedgehog_Dilemma9#MoveAway"/>
        <owl:differentFrom rdf:resource="http://www.semanticweb.org/walte/ontologies/2024/5/Hedgehog_Dilemma9#ProperDistance"/>
        <Hedgehog_Dilemma9:hasCriterion rdf:resource="http://www.semanticweb.org/walte/ontologies/2024/5/Hedgehog_Dilemma9#Interdependence"/>
    </owl:NamedIndividual>
    


    <!-- http://www.semanticweb.org/walte/ontologies/2024/5/Hedgehog_Dilemma9#GetHurt -->

    <owl:NamedIndividual rdf:about="http://www.semanticweb.org/walte/ontologies/2024/5/Hedgehog_Dilemma9#GetHurt">
        <rdf:type rdf:resource="http://www.ontologydesignpatterns.org/cp/owl/controlflow.owl#DecisionActivity"/>
        <owl:differentFrom rdf:resource="http://www.semanticweb.org/walte/ontologies/2024/5/Hedgehog_Dilemma9#MoveCloser"/>
        <sequence:follows rdf:resource="http://www.semanticweb.org/walte/ontologies/2024/5/Hedgehog_Dilemma9#MoveCloser"/>
        <sequence:precedes rdf:resource="http://www.semanticweb.org/walte/ontologies/2024/5/Hedgehog_Dilemma9#BeingAlone_and_Pain"/>
        <dc:creator>Walter Bertoli</dc:creator>
        <rdfs:comment>When it get in contact with the other hedgehogs, the quills cause the hedgehog to get hurt</rdfs:comment>
    </owl:NamedIndividual>
    


    <!-- http://www.semanticweb.org/walte/ontologies/2024/5/Hedgehog_Dilemma9#HedgehogProblem -->

    <owl:NamedIndividual rdf:about="http://www.semanticweb.org/walte/ontologies/2024/5/Hedgehog_Dilemma9#HedgehogProblem">
        <rdf:type rdf:resource="http://www.ontologydesignpatterns.org/ont/dilemmas/coredilemma.owl#Dilemma"/>
        <dc:creator>Walter Bertoli</dc:creator>
    </owl:NamedIndividual>
    


    <!-- http://www.semanticweb.org/walte/ontologies/2024/5/Hedgehog_Dilemma9#Individualism -->

    <owl:NamedIndividual rdf:about="http://www.semanticweb.org/walte/ontologies/2024/5/Hedgehog_Dilemma9#Individualism">
        <rdf:type rdf:resource="http://www.semanticweb.org/walte/ontologies/2024/5/Hedgehog_Dilemma9#Individualism"/>
        <owl:differentFrom rdf:resource="http://www.semanticweb.org/walte/ontologies/2024/5/Hedgehog_Dilemma9#Interdependence"/>
        <owl:differentFrom rdf:resource="http://www.semanticweb.org/walte/ontologies/2024/5/Hedgehog_Dilemma9#Kindness"/>
        <descriptionandsituation:describes rdf:resource="http://www.semanticweb.org/walte/ontologies/2024/5/Hedgehog_Dilemma#Hedgehog1"/>
        <coredilemma:hasOutcome rdf:resource="http://www.semanticweb.org/walte/ontologies/2024/5/Hedgehog_Dilemma9#MoveAway"/>
    </owl:NamedIndividual>
    


    <!-- http://www.semanticweb.org/walte/ontologies/2024/5/Hedgehog_Dilemma9#Interdependence -->

    <owl:NamedIndividual rdf:about="http://www.semanticweb.org/walte/ontologies/2024/5/Hedgehog_Dilemma9#Interdependence">
        <rdf:type rdf:resource="http://www.semanticweb.org/walte/ontologies/2024/5/Hedgehog_Dilemma9#Interdependence"/>
        <owl:differentFrom rdf:resource="http://www.semanticweb.org/walte/ontologies/2024/5/Hedgehog_Dilemma9#Kindness"/>
        <descriptionandsituation:describes rdf:resource="http://www.semanticweb.org/walte/ontologies/2024/5/Hedgehog_Dilemma#Hedgehog2"/>
        <coredilemma:hasOutcome rdf:resource="http://www.semanticweb.org/walte/ontologies/2024/5/Hedgehog_Dilemma9#GetCloser"/>
    </owl:NamedIndividual>
    


    <!-- http://www.semanticweb.org/walte/ontologies/2024/5/Hedgehog_Dilemma9#Kindness -->

    <owl:NamedIndividual rdf:about="http://www.semanticweb.org/walte/ontologies/2024/5/Hedgehog_Dilemma9#Kindness">
        <rdf:type rdf:resource="http://www.semanticweb.org/walte/ontologies/2024/5/Hedgehog_Dilemma9#Kindness"/>
        <coredilemma:hasOutcome rdf:resource="http://www.semanticweb.org/walte/ontologies/2024/5/Hedgehog_Dilemma9#ProperDistance"/>
    </owl:NamedIndividual>
    


    <!-- http://www.semanticweb.org/walte/ontologies/2024/5/Hedgehog_Dilemma9#MoveAway -->

    <owl:NamedIndividual rdf:about="http://www.semanticweb.org/walte/ontologies/2024/5/Hedgehog_Dilemma9#MoveAway">
        <rdf:type rdf:resource="http://www.semanticweb.org/walte/ontologies/2024/5/Hedgehog_Dilemma9#MoveAway"/>
        <owl:differentFrom rdf:resource="http://www.semanticweb.org/walte/ontologies/2024/5/Hedgehog_Dilemma9#ProperDistance"/>
        <Hedgehog_Dilemma9:hasCriterion rdf:resource="http://www.semanticweb.org/walte/ontologies/2024/5/Hedgehog_Dilemma9#Individualism"/>
    </owl:NamedIndividual>
    


    <!-- http://www.semanticweb.org/walte/ontologies/2024/5/Hedgehog_Dilemma9#MoveCloser -->

    <owl:NamedIndividual rdf:about="http://www.semanticweb.org/walte/ontologies/2024/5/Hedgehog_Dilemma9#MoveCloser">
        <rdf:type rdf:resource="http://www.ontologydesignpatterns.org/cp/owl/controlflow.owl#DecisionActivity"/>
        <sequence:follows rdf:resource="http://www.semanticweb.org/walte/ontologies/2024/5/Hedgehog_Dilemma9#Coldness"/>
        <sequence:precedes rdf:resource="http://www.semanticweb.org/walte/ontologies/2024/5/Hedgehog_Dilemma9#GetHurt"/>
        <dc:creator>Walter Bertoli</dc:creator>
        <rdfs:comment>The Hedgehog looks for heat, moveing closer to the other animals.</rdfs:comment>
    </owl:NamedIndividual>
    


    <!-- http://www.semanticweb.org/walte/ontologies/2024/5/Hedgehog_Dilemma9#ProperDistance -->

    <owl:NamedIndividual rdf:about="http://www.semanticweb.org/walte/ontologies/2024/5/Hedgehog_Dilemma9#ProperDistance">
        <rdf:type rdf:resource="http://www.semanticweb.org/walte/ontologies/2024/5/Hedgehog_Dilemma9#ProperDistance"/>
        <Hedgehog_Dilemma9:hasCriterion rdf:resource="http://www.semanticweb.org/walte/ontologies/2024/5/Hedgehog_Dilemma9#Kindness"/>
    </owl:NamedIndividual>
    


    <!-- 
    ///////////////////////////////////////////////////////////////////////////////////////
    //
    // Annotations
    //
    ///////////////////////////////////////////////////////////////////////////////////////
     -->

    <rdf:Description rdf:about="http://www.semanticweb.org/walte/ontologies/2024/5/Hedgehog_Dilemma9#GetCloser">
        <dc:creator>Walter Bertoli</dc:creator>
        <rdfs:comment>Get closer to the other Hedgehogs</rdfs:comment>
    </rdf:Description>
    <rdf:Description rdf:about="http://www.semanticweb.org/walte/ontologies/2024/5/Hedgehog_Dilemma9#Individualism">
        <dc:creator>Walter Bertoli</dc:creator>
        <rdfs:comment>The Hedgehog chooses to preseve itself, going away from others</rdfs:comment>
    </rdf:Description>
    <rdf:Description rdf:about="http://www.semanticweb.org/walte/ontologies/2024/5/Hedgehog_Dilemma9#Interdependence">
        <dc:creator>Walter Bertoli</dc:creator>
        <rdfs:comment>The Hedgehog needs other forms of life, so it chooses to be near its similars, in spite of the pain</rdfs:comment>
    </rdf:Description>
    <rdf:Description rdf:about="http://www.semanticweb.org/walte/ontologies/2024/5/Hedgehog_Dilemma9#Kindness">
        <dc:creator>Walter Bertoli</dc:creator>
        <rdfs:comment>The Hedgehog chooses politeness: it will not be the closest possible so it will not fell complete warm, but he tries to find a right distance to not fell the pain</rdfs:comment>
    </rdf:Description>
    <rdf:Description rdf:about="http://www.semanticweb.org/walte/ontologies/2024/5/Hedgehog_Dilemma9#MoveAway">
        <dc:creator>Walter Bertoli</dc:creator>
        <rdfs:comment>Move away from the other Hedgehogs</rdfs:comment>
    </rdf:Description>
    <rdf:Description rdf:about="http://www.semanticweb.org/walte/ontologies/2024/5/Hedgehog_Dilemma9#ProperDistance">
        <dc:creator>Walter Bertoli</dc:creator>
        <rdfs:comment>Keep the proper distance from the other Hedgehogs</rdfs:comment>
    </rdf:Description>
</rdf:RDF>



<!-- Generated by the OWL API (version 4.5.26.2023-07-17T20:34:13Z) https://github.com/owlcs/owlapi -->

